List equality proofs

Core_Erlang_Environment.v
@@ -21,52 +21,19 @@ match env with
 end.
 
 (** Get *)
-Fixpoint get_value (env : Environment) (key : (Var + FunctionIdentifier)) : (Value + Exception) :=
+Fixpoint get_value (env : Environment) (key : (Var + FunctionIdentifier)) 
+   : (Value + Exception) :=
 match env with
 | [ ] => inr novar
 | (k,v)::xs => if uequal key k then inl v else get_value xs key
 end.
 
-Fixpoint insert_value (env : Environment) (key : (Var + FunctionIdentifier)) (value : Value) :=
+Fixpoint insert_value (env : Environment) (key : (Var + FunctionIdentifier)) 
+   (value : Value) : Environment :=
 match env with
   | [] => [(key, value)]
   | (k,v)::xs => if uequal k key then (key,value)::xs else (k,v)::(insert_value xs key value)
 end.
-
-(** Set with overwrite *)
-(* Fixpoint insert_closure (env : Environment) (key : (Var + FunctionIdentifier)) (value : Value) (count : nat) : Environment :=
-match value with
-| VClosure def ext n ps b =>
-  match env with
-  | [] => [(key, VClosure def ext count ps b)]
-  | (k,v)::xs => if uequal k key 
-                 then match v with
-                      | VClosure _ _ n _ _ => (key, VClosure def ext n ps b)::xs
-                      | _ => (key, VClosure def ext count ps b)::xs
-                      end
-                 else (k,v)::(insert_value xs key value count)
-  end
-| _ =>
-  match env with
-  | [] => [(key, value)]
-  | (k,v)::xs => if uequal k key then (key,value)::xs else (k,v)::(insert_value xs key value count)
-  end
-end. *)
-
-(** Set without overwrite *)
-(* Fixpoint insert_value_no_overwrite (env : Environment) (key : (Var + FunctionIdentifier)) (value : Value) : Environment :=
-match env with
-| [] => [(key, value)]
-| (k,v)::xs => if uequal k key then env else (k,v)::(insert_value xs key value)
-end.
- *)
-
-(* Merge environments *)
-(* Fixpoint env_fold (e1 e2: Environment) : Environment :=
-match e1 with
-| [] => e2
-| (k,v)::xs => env_fold xs (insert_value e2 k v)
-end. *)
 
 (** Add additional bindings *)
 (** We used here: when binding, variables must be unique *)
@@ -77,7 +44,8 @@ match bindings with
 end.
 
 (** Add bindings with two lists *)
-Fixpoint append_vars_to_env (vl : list Var) (el : list Value) (d : Environment) : Environment :=
+Fixpoint append_vars_to_env (vl : list Var) (el : list Value) (d : Environment) 
+   : Environment :=
 match vl, el with
 | [], [] => d
 | v::vs, e::es => append_vars_to_env vs es (insert_value d (inl v) e)
@@ -87,43 +55,44 @@ end.
 (** Not Overwriting insert *)
 (** Overwriting does not fit with this recursion *)
 Fixpoint insert_function (id : nat) (v : FunctionIdentifier) (p : list Var) (b : Expression) 
- (l : list (nat * FunctionIdentifier * FunctionExpression)) : list (nat * FunctionIdentifier * FunctionExpression) :=
+   (l : list (nat * FunctionIdentifier * FunctionExpression)) 
+    : list (nat * FunctionIdentifier * FunctionExpression) :=
 match l with
 | [] => [(id, v, (p, b))]
-| (id', k, v0)::xs => if equal k v then (id', k, v0)::xs else (id', k, v0)::(insert_function id v p b xs)
+| (id', k, v0)::xs => if equal k v then (id', k, v0)::xs 
+                                   else (id', k, v0)::(insert_function id v p b xs)
 end.
 
 (** Lists represented functions *)
 Fixpoint list_functions (vl : list FunctionIdentifier) (paramss : list (list Var)) 
-      (bodies : list Expression) (last_id : nat) : list (nat * FunctionIdentifier * FunctionExpression) :=
+      (bodies : list Expression) (last_id : nat) 
+      : list (nat * FunctionIdentifier * FunctionExpression) :=
 match vl, paramss, bodies with
 | [], [], [] => []
-| v::vs, varl::ps, e::bs => insert_function last_id v varl e (list_functions vs ps bs (S last_id))
+| v::vs, varl::ps, e::bs => insert_function last_id v varl e 
+                                 (list_functions vs ps bs (S last_id))
 | _, _, _ => []
 end.
-
-(* (** Inserting closures *)
-Fixpoint insert_closure (name : FunctionIdentifier) (env def : Environment) (deffuns : list (FunctionIdentifier * FunctionExpression)) (params : list Var) (count : nat)
-      (body :  Expression) : Environment :=
-match env with
-| [] => [(inr name, VClosure def deffuns count varl e)]
-| (k,v)::xs => if uequal k (inr name) then (key,value)::xs else (k,v)::(insert_value xs key value)
-end. *)
 
 (** Add functions *)
 Fixpoint append_funs_to_env_base (vl : list FunctionIdentifier) (paramss : list (list Var)) 
       (bodies : list Expression) (d : Environment) (def : Environment) 
-      (deffuns : list (nat * FunctionIdentifier * FunctionExpression)) (last_id : nat) : Environment :=
+      (deffuns : list (nat * FunctionIdentifier * FunctionExpression)) (last_id : nat) 
+      : Environment :=
 match vl, paramss, bodies with
 | [], [], [] => d
 | v::vs, varl::ps, e::bs => append_funs_to_env_base vs ps bs 
-                              (insert_value d (inr v) (VClosure def deffuns last_id varl e)) def deffuns (S last_id)
+                              (insert_value d (inr v) 
+                                           (VClosure def deffuns last_id varl e)) 
+                                           def deffuns (S last_id)
 | _, _, _ => []
 end.
 
 Definition append_funs_to_env (vl : list FunctionIdentifier) (paramss : list (list Var)) 
       (bodies : list Expression) (d : Environment) (last_id : nat) : Environment :=
-append_funs_to_env_base vl paramss bodies d d (list_functions vl paramss bodies last_id) last_id
+append_funs_to_env_base vl paramss bodies d d 
+                       (list_functions vl paramss bodies last_id)
+                       last_id
 .
 
 (** Examples *)
@@ -142,14 +111,16 @@ Compute insert_function 2 ("f1"%string, 0) [] ErrorExp (list_functions
                               [ErrorExp; ErrorExp; ErrorExp] 0).
 
 (** Environment construction from the extension and the reference *)
-Fixpoint get_env_base (env def : Environment) (ext defext : list (nat * FunctionIdentifier * FunctionExpression))
+Fixpoint get_env_base (env def : Environment) 
+   (ext defext : list (nat * FunctionIdentifier * FunctionExpression))
    : Environment :=
 match ext with
 | [] => env
 | (id, f1, (pl, b))::xs => get_env_base (insert_value env (inr f1) (VClosure def defext id pl b)) def xs defext
 end.
 
-Definition get_env (env : Environment) (ext : list (nat * FunctionIdentifier * FunctionExpression))
+Definition get_env (env : Environment) 
+   (ext : list (nat * FunctionIdentifier * FunctionExpression))
    : Environment :=
   get_env_base env env ext ext
 .
