Core_Erlang_Semantics.v
@@ -54,7 +54,7 @@ Inductive eval_expr : Environment -> nat -> Expression -> SideEffectList -> nat 
 | eval_var (env:Environment) (s: Var) (eff : SideEffectList) (id : nat) :
   |env, id, EVar s, eff| -e> |id, get_value env (inl s), eff|
 
-(* Function Signature evaluation rule *)
+(* Function identifier evaluation rule *)
 | eval_funid (env:Environment) (fid : FunctionIdentifier) (eff : SideEffectList) (id : nat):
   |env, id, EFunId fid, eff| -e> |id, get_value env (inr fid), eff|
 
@@ -64,7 +64,7 @@ Inductive eval_expr : Environment -> nat -> Expression -> SideEffectList -> nat 
 
 (* tuple evaluation rule *)
 | eval_tuple (env: Environment) (exps : list Expression) (vals : list Value) 
-     (eff1 eff2 : SideEffectList) (eff : list SideEffectList) (ids : list nat) (id : nat) :
+     (eff1 eff2 : SideEffectList) (eff : list SideEffectList) (ids : list nat) (id id' : nat) :
   length exps = length vals ->
   length exps = length eff ->
   length exps = length ids ->
@@ -74,9 +74,10 @@ Inductive eval_expr : Environment -> nat -> Expression -> SideEffectList -> nat 
      -e> 
       |nth_id ids id (S i), inl (nth i vals ErrorValue), concatn eff1 eff (S i)|
   ) ->
-  eff2 = concatn eff1 eff (length vals)
+  eff2 = concatn eff1 eff (length vals) ->
+  id' = last ids id (* if length = 0, then last id = first id *)
 ->
-  |env, id, ETuple exps, eff1| -e> |last ids 0, inl (VTuple vals), eff2|
+  |env, id, ETuple exps, eff1| -e> |id' , inl (VTuple vals), eff2|
 
 (* list evaluation rule *)
 | eval_list (env:Environment) (hd tl: Expression) (hdv tlv : Value) 
@@ -90,7 +91,8 @@ Inductive eval_expr : Environment -> nat -> Expression -> SideEffectList -> nat 
 (* case evaluation rules *)
 | eval_case (env: Environment) (e guard exp: Expression) (v : Value) (v' : Value + Exception) 
      (patts : list Pattern) (guards : list Expression) (bodies : list Expression) 
-     (bindings: list (Var * Value)) (i : nat) (eff1 eff2 eff3 eff4 : SideEffectList) (id id' id'' : nat) :
+     (bindings: list (Var * Value)) (i : nat) (eff1 eff2 eff3 eff4 : SideEffectList) 
+     (id id' id'' : nat) :
   length patts = length guards ->
   length patts = length bodies ->
   |env, id, e, eff1| -e> |id', inl v, eff1 ++ eff2| ->
@@ -114,7 +116,8 @@ Inductive eval_expr : Environment -> nat -> Expression -> SideEffectList -> nat 
 
 (* call evaluation rule *)
 | eval_call (env: Environment) (v : Value + Exception) (params : list Expression) 
-     (vals : list Value) (fname: string) (eff1 eff2: SideEffectList) (eff : list SideEffectList) (ids : list nat) (id : nat) :
+     (vals : list Value) (fname: string) (eff1 eff2: SideEffectList) (eff : list SideEffectList) 
+     (ids : list nat) (id id' : nat) :
   length params = length vals ->
   length params = length eff ->
   length params = length ids ->
@@ -124,15 +127,17 @@ Inductive eval_expr : Environment -> nat -> Expression -> SideEffectList -> nat 
      -e>
       |nth_id ids id (S i), inl (nth i vals ErrorValue), concatn eff1 eff (S i)|
   ) ->
-  eval fname vals (concatn eff1 eff (length params)) = (v, eff2)
+  eval fname vals (concatn eff1 eff (length params)) = (v, eff2) ->
+  id' = last ids id
 ->
-  |env, id, ECall fname params, eff1| -e> |last ids 0, v, eff2|
+  |env, id, ECall fname params, eff1| -e> |id', v, eff2|
 
 (* apply functions*)
 | eval_apply (params : list Expression) (vals : list Value) (env : Environment) 
      (exp : Expression) (body : Expression) (v : Value + Exception) (var_list : list Var) 
      (ref : Environment) (ext : list (nat * FunctionIdentifier * FunctionExpression)) 
-     (eff1 eff2 eff3 eff4 : SideEffectList) (eff : list SideEffectList) (n : nat) (ids : list nat) (id id' id'' : nat) :
+     (eff1 eff2 eff3 eff4 : SideEffectList) (eff : list SideEffectList) (n : nat) 
+     (ids : list nat) (id id' id'' : nat) :
   length params = length vals ->
   |env, id, exp, eff1| -e> |id', inl (VClosure ref ext n var_list body), eff1 ++ eff2| ->
   length var_list = length vals
@@ -149,7 +154,7 @@ Inductive eval_expr : Environment -> nat -> Expression -> SideEffectList -> nat 
   eff4 = concatn (eff1 ++ eff2) eff (length params) ++ eff3
   ->
   |append_vars_to_env var_list vals (get_env ref ext), 
-   last ids 0,
+   last ids id',
    body, 
    concatn (eff1 ++ eff2) eff (length params)|
   -e>
@@ -173,7 +178,9 @@ Inductive eval_expr : Environment -> nat -> Expression -> SideEffectList -> nat 
   ->
     eff3 = concatn eff1 eff (length exps) ++ eff2
   ->
-    |append_vars_to_env vars vals env, last ids 0, e, concatn eff1 eff (length exps)| -e> |id', v, eff3|
+    |append_vars_to_env vars vals env, last ids id, e, concatn eff1 eff (length exps)| 
+    -e> 
+    |id', v, eff3|
 ->
   |env, id, ELet vars exps e, eff1| -e> |id', v, eff3|
 
@@ -198,7 +205,7 @@ Inductive eval_expr : Environment -> nat -> Expression -> SideEffectList -> nat 
 
 (* map evaluation rule *)
 | eval_map (kl vl: list Expression) (vvals kvals kl' vl' : list Value) (env: Environment) 
-     (eff1 eff2 : SideEffectList) (eff : list SideEffectList) (id : nat) (ids : list nat) :
+     (eff1 eff2 : SideEffectList) (eff : list SideEffectList) (id id' : nat) (ids : list nat) :
   length kl = length vl ->
   length kl = length vvals ->
   length kl = length kvals ->
@@ -217,9 +224,10 @@ Inductive eval_expr : Environment -> nat -> Expression -> SideEffectList -> nat 
    -e>
     |nth_id ids id (S (S (2 * i))),inl (nth i vvals ErrorValue), concatn eff1 eff (S (S (2*i)))|
   ) ->
-  eff2 = concatn eff1 eff ((length kvals) * 2)
+  eff2 = concatn eff1 eff ((length kvals) * 2) ->
+  id' = last ids id
 ->
-  |env, id, EMap kl vl, eff1| -e> |last ids 0, inl (VMap kl' vl'), eff2|
+  |env, id, EMap kl vl, eff1| -e> |id', inl (VMap kl' vl'), eff2|
 
 
   (* EXCEPTIONS *)
@@ -242,7 +250,8 @@ Inductive eval_expr : Environment -> nat -> Expression -> SideEffectList -> nat 
 
 (* tuple exception *)
 | eval_tuple_ex (env: Environment) (i : nat) (exps : list Expression) (vals : list Value) 
-     (ex : Exception) (eff1 eff2 eff3 : SideEffectList) (eff : list SideEffectList) (id id' : nat) (ids : list nat) :
+     (ex : Exception) (eff1 eff2 eff3 : SideEffectList) (eff : list SideEffectList) 
+     (id id' : nat) (ids : list nat) :
   length vals = i ->
   i < length exps ->
   length eff = i ->
@@ -252,14 +261,15 @@ Inductive eval_expr : Environment -> nat -> Expression -> SideEffectList -> nat 
    -e>
     |nth_id ids id (S j), inl (nth j vals ErrorValue), concatn eff1 eff (S j)|) ->
   eff3 = concatn eff1 eff i ++ eff2 ->
-  |env, last ids 0, nth i exps ErrorExp, concatn eff1 eff i| -e> |id', inr ex, eff3|
+  |env, last ids id, nth i exps ErrorExp, concatn eff1 eff i| -e> |id', inr ex, eff3|
 ->
   |env, id, ETuple exps, eff1| -e> |id', inr ex, eff3|
 
 
 (* try 2x *)
-| eval_try (env: Environment) (e e1 e2 : Expression) (v vex1 vex2 vex3 : Var) (val : Value + Exception) 
-      (val' : Value) (eff1 eff2 eff3 eff4 : SideEffectList) (id id' id'' : nat) :
+| eval_try (env: Environment) (e e1 e2 : Expression) (v vex1 vex2 vex3 : Var) 
+      (val : Value + Exception) (val' : Value) (eff1 eff2 eff3 eff4 : SideEffectList)
+      (id id' id'' : nat) :
   |env, id, e, eff1| -e> |id', inl val', eff1 ++ eff2| ->
   eff4 = eff1 ++ eff2 ++ eff3 ->
   |append_vars_to_env [v] [val'] env, id', e1, eff1 ++ eff2| -e> |id'', val, eff4|
@@ -267,7 +277,8 @@ Inductive eval_expr : Environment -> nat -> Expression -> SideEffectList -> nat 
   |env, id, ETry e e1 e2 v vex1 vex2 vex3, eff1| -e> |id'', val, eff4|
 
 | eval_try_catch (env: Environment) (e e1 e2 : Expression) (v vex1 vex2 vex3 : Var) 
-      (val : Value + Exception) (ex : Exception) (eff1 eff2 eff3 eff4 : SideEffectList) (id id' id'' : nat) :
+      (val : Value + Exception) (ex : Exception) (eff1 eff2 eff3 eff4 : SideEffectList) 
+      (id id' id'' : nat) :
   |env, id, e, eff1| -e> |id', inr ex, eff1 ++ eff2| ->
   eff4 = eff1 ++ eff2 ++ eff3 ->
   |append_vars_to_env [vex1; vex2; vex3] 
@@ -282,7 +293,8 @@ Inductive eval_expr : Environment -> nat -> Expression -> SideEffectList -> nat 
 (* case 2x *)
 (** Pattern matching exception *)
 | eval_case_ex_pat (env: Environment) (e : Expression) (ex : Exception) (patterns : list Pattern) 
-     (guards : list Expression) (bodies : list Expression)  (eff1 eff2 eff3 : SideEffectList) (id id' : nat):
+     (guards : list Expression) (bodies : list Expression)  (eff1 eff2 eff3 : SideEffectList) 
+     (id id' : nat):
   length patterns = length guards ->
   length patterns = length bodies ->
   eff3 = eff1 ++ eff2 ->
@@ -292,7 +304,8 @@ Inductive eval_expr : Environment -> nat -> Expression -> SideEffectList -> nat 
 
 (** No matching clause *)
 | eval_case_clause_ex (env: Environment) (e : Expression) (patterns : list Pattern) 
-     (guards : list Expression) (bodies : list Expression) (v : Value) (eff1 eff2 eff3 : SideEffectList) (id id' : nat):
+     (guards : list Expression) (bodies : list Expression) (v : Value) 
+     (eff1 eff2 eff3 : SideEffectList) (id id' : nat):
   length patterns = length guards ->
   length patterns = length bodies ->
   eff3 = eff1 ++ eff2 ->
@@ -309,25 +322,11 @@ Inductive eval_expr : Environment -> nat -> Expression -> SideEffectList -> nat 
 ->
 |env, id, ECase e patterns guards bodies, eff1| -e> |id', inr (if_clause v), eff3|
 (** ith guard exception -> guards cannot result in exception, i.e. this rule is not needed *)
-(* | eval_case_ex_guard (env: Environment) (e e'' guard exp: Expression) (v : Value) (ex : Exception) (patterns : list Pattern) (guards : list Expression) (bodies : list Expression) (bindings: list (Var * Value)) (i : nat) (eff1 eff2 eff3 : SideEffectList):
-  length patterns = length guards ->
-  length patterns = length bodies ->
-  eff3 = eff1 ++ eff2 ->
-  |env, e, eff1| -e> |inl v, eff3| ->
-  match_clause v patterns guards bodies i = Some (guard, exp, bindings) ->
-  (forall j : nat, j < i -> 
-
-    (forall gg ee bb, match_clause v patterns guards bodies j = Some (gg, ee, bb) -> ((|add_bindings bb env, gg, eff3| -e> |inl ffalse, eff3| )))
-
-  ) ->
-  |add_bindings bindings env, guard, eff3| -e> |inr ex, eff3|
-->
-  |env, ECase e patterns guards bodies, eff1| -e> |inr ex, eff3| *)
-
 
 (* call 1x *)
 | eval_call_ex (env: Environment) (i : nat) (fname : string) (params : list Expression) 
-     (vals : list Value) (ex : Exception) (eff1 eff2 eff3 : SideEffectList) (eff : list SideEffectList) (id : nat) (ids : list nat) :
+     (vals : list Value) (ex : Exception) (eff1 eff2 eff3 : SideEffectList) 
+     (eff : list SideEffectList) (id id' : nat) (ids : list nat) :
   length vals = i ->
   i < length params ->
   length eff = i ->
@@ -338,10 +337,10 @@ Inductive eval_expr : Environment -> nat -> Expression -> SideEffectList -> nat 
     |nth_id ids id (S j), inl (nth j vals ErrorValue), concatn eff1 eff (S j)|
   ) ->
   eff3 = concatn eff1 eff i ++ eff2 ->
-  |env, id, nth i params ErrorExp, concatn eff1 eff i| -e> |last ids 0, inr ex, eff3|
+  |env, last ids id, nth i params ErrorExp, concatn eff1 eff i| -e> |id', inr ex, eff3|
 
 ->
-  |env, id, ECall fname params, eff1| -e> |last ids 0, inr ex, eff3|
+  |env, id, ECall fname params, eff1| -e> |id', inr ex, eff3|
 
 (* apply 4x *)
 (** According to ref. implementation, here it is not needed to check the arg number *)
@@ -370,13 +369,14 @@ Inductive eval_expr : Environment -> nat -> Expression -> SideEffectList -> nat 
     |nth_id ids id' (S j), inl (nth j vals ErrorValue), concatn (eff1 ++ eff2) eff (S j)|
   ) ->
   eff4 = concatn (eff1 ++ eff2) eff i ++ eff3 ->
-  |env, last ids 0, nth i params ErrorExp, concatn (eff1 ++ eff2) eff i| -e> |id'', inr ex, eff4|
+  |env, last ids id', nth i params ErrorExp, concatn (eff1 ++ eff2) eff i| -e> |id'', inr ex, eff4|
 ->
   |env, id, EApply exp params, eff1| -e> |id'', inr ex, eff4|
 
 (** Then we check if the name expression evaluates to a closure *)
 | eval_apply_ex_closure (params : list Expression) (vals: list Value) (env : Environment) (v : Value) 
-     (exp : Expression) (eff1 eff2 eff3 : SideEffectList) (eff : list SideEffectList) (ids : list nat) (id id' : nat):
+     (exp : Expression) (eff1 eff2 eff3 : SideEffectList) (eff : list SideEffectList) 
+     (ids : list nat) (id id' id'' : nat):
   length params = length vals ->
   length params = length eff ->
   length params = length ids ->
@@ -384,22 +384,23 @@ Inductive eval_expr : Environment -> nat -> Expression -> SideEffectList -> nat 
   (
     forall j : nat, j < length params ->
     (
-      |env, nth_id ids id j, nth j params ErrorExp, concatn (eff1 ++ eff2) eff j|
+      |env, nth_id ids id' j, nth j params ErrorExp, concatn (eff1 ++ eff2) eff j|
      -e>
-      |nth_id ids id (S j), inl (nth j vals ErrorValue), concatn (eff1 ++ eff2) eff (S j)|
+      |nth_id ids id' (S j), inl (nth j vals ErrorValue), concatn (eff1 ++ eff2) eff (S j)|
     )
   ) ->
   (forall ref ext var_list body n, 
      v <> VClosure ref ext n var_list body) ->
-  eff3 = concatn (eff1 ++ eff2) eff (length params)
+  eff3 = concatn (eff1 ++ eff2) eff (length params) ->
+  id'' = last ids id'
 ->
-  |env, id, EApply exp params, eff1| -e> |last ids 0, inr (badfun v), eff3|
+  |env, id, EApply exp params, eff1| -e> |id'', inr (badfun v), eff3|
 
 (** too few or too many arguments are given *)
 | eval_apply_ex_param_count (params : list Expression) (vals : list Value) (env : Environment) 
      (exp : Expression) (body : Expression) (var_list : list Var) (ref : Environment) 
      (ext : list (nat * FunctionIdentifier * FunctionExpression)) (eff1 eff2 eff3 : SideEffectList) 
-     (eff : list SideEffectList) (n : nat) (ids : list nat) (id id' : nat):
+     (eff : list SideEffectList) (n : nat) (ids : list nat) (id id' id'' : nat):
   length params = length vals ->
   length params = length eff ->
   length params = length ids ->
@@ -407,15 +408,18 @@ Inductive eval_expr : Environment -> nat -> Expression -> SideEffectList -> nat 
   (
     forall j : nat, j < length params ->
     (
-      |env, nth_id ids id j, nth j params ErrorExp, concatn (eff1 ++ eff2) eff j|
+      |env, nth_id ids id' j, nth j params ErrorExp, concatn (eff1 ++ eff2) eff j|
      -e>
-      |nth_id ids id (S j), inl (nth j vals ErrorValue), concatn (eff1 ++ eff2) eff (S j)|
+      |nth_id ids id' (S j), inl (nth j vals ErrorValue), concatn (eff1 ++ eff2) eff (S j)|
     )
   ) ->
   length var_list <> length vals ->
-  eff3 = concatn (eff1 ++ eff2) eff (length params)
+  eff3 = concatn (eff1 ++ eff2) eff (length params) ->
+  id'' = last ids id'
 ->
-  |env, id, EApply exp params, eff1| -e> |last ids 0, inr (badarity (VClosure ref ext n var_list body)), eff3|
+  |env, id, EApply exp params, eff1| 
+  -e> 
+  |id'', inr (badarity (VClosure ref ext n var_list body)), eff3|
 
 (* let 1x *)
 | eval_let_ex_param (env: Environment) (exps: list Expression) (vals : list Value) (vars: list Var) 
@@ -431,14 +435,15 @@ Inductive eval_expr : Environment -> nat -> Expression -> SideEffectList -> nat 
     |nth_id ids id (S j), inl (nth j vals ErrorValue), concatn eff1 eff (S j)|
   ) ->
   eff3 = concatn eff1 eff i ++ eff2 ->
-  |env, last ids 0, nth i exps ErrorExp, concatn eff1 eff i| -e> |id', inr ex, eff3|
+  |env, last ids id, nth i exps ErrorExp, concatn eff1 eff i| -e> |id', inr ex, eff3|
 ->
   |env, id, ELet vars exps e, eff1| -e> |id', inr ex, eff3|
 
 (* map 2x *)
 (** Exception in key list *)
 | eval_map_ex_key (kl vl: list Expression) (vvals kvals : list Value) (env: Environment) (i : nat) 
-     (ex : Exception) (eff1 eff2 eff3 : SideEffectList) (eff : list SideEffectList) (ids : list nat) (id id' : nat):
+     (ex : Exception) (eff1 eff2 eff3 : SideEffectList) (eff : list SideEffectList) 
+     (ids : list nat) (id id' : nat):
   length kl = length vl ->
   length vvals = i ->
   length kvals = i ->
@@ -460,13 +465,14 @@ Inductive eval_expr : Environment -> nat -> Expression -> SideEffectList -> nat 
   )
   ->
   eff3 = concatn eff1 eff (2 * i) ++ eff2 ->
-  |env, last ids 0, nth i kl ErrorExp, concatn eff1 eff (2 * i)| -e> |id', inr ex, eff3|
+  |env, last ids id, nth i kl ErrorExp, concatn eff1 eff (2 * i)| -e> |id', inr ex, eff3|
 ->
   |env, id, EMap kl vl, eff1| -e> |id', inr ex, eff3|
 
 (** Exception in value list *)
 | eval_map_ex_val (kl vl: list Expression) (vvals kvals : list Value) (env: Environment) (i : nat) 
-     (ex : Exception) (val : Value) (eff1 eff2 eff3 eff4 : SideEffectList) (eff : list SideEffectList) (ids : list nat) (id id' id'' : nat):
+     (ex : Exception) (val : Value) (eff1 eff2 eff3 eff4 : SideEffectList) 
+     (eff : list SideEffectList) (ids : list nat) (id id' id'' : nat):
   length kl = length vl ->
   length vvals = i ->
   length kvals = i ->
@@ -485,11 +491,13 @@ Inductive eval_expr : Environment -> nat -> Expression -> SideEffectList -> nat 
    -e>
     |nth_id ids id (S (S (2*j))), inl (nth j vvals ErrorValue), concatn eff1 eff (S (S (2 * j)))|
   )
-  ->
-  |env, last ids 0, nth i kl ErrorExp, concatn eff1 eff (2 * i)| -e> |id', inl val, concatn eff1 eff (2 * i) ++ eff2|
-  ->
+ ->
+  |env, last ids id, nth i kl ErrorExp, concatn eff1 eff (2 * i)| 
+  -e> 
+  |id', inl val, concatn eff1 eff (2 * i) ++ eff2|
+ ->
   eff4 = concatn eff1 eff (2 * i) ++ eff2 ++ eff3
-  ->
+ ->
   |env, id', nth i vl ErrorExp, concatn eff1 eff (2 * i) ++ eff2| -e> |id'', inr ex, eff4|
 ->
   |env, id, EMap kl vl, eff1| -e> |id'', inr ex, eff4|
@@ -502,7 +510,8 @@ where "| env , id , e , eff | -e> | id' , e' , eff' |" := (eval_expr env id e ef
 (* Fixpoint add_elements_to_env (fl : list ErlFunction) : Environment :=
 match fl with
 | [] => []
-| (TopLevelFun sig (vl,exp))::xs => insert_value_no_overwrite (add_elements_to_env xs) (inr sig) (VClosure (inr sig) vl exp)
+| (TopLevelFun sig (vl,exp))::xs => insert_value_no_overwrite 
+                                    (add_elements_to_env xs) (inr sig) (VClosure (inr sig) vl exp)
 end.
 
 Fixpoint initialize_proving (module : ErlModule) : Environment :=
@@ -513,7 +522,8 @@ end.
 Fixpoint add_elements_to_closure (fl : list ErlFunction) (module : ErlModule) : Closures :=
 match fl with
 | [] => []
-| (TopLevelFun sig f)::xs => set_closure_no_overwrite (add_elements_to_closure xs module) sig (initialize_proving module)
+| (TopLevelFun sig f)::xs => set_closure_no_overwrite (add_elements_to_closure xs module) sig 
+                            (initialize_proving module)
 end.
 
 Fixpoint initialize_proving_closures (module : ErlModule) : Closures :=
